\documentclass{article}

\usepackage[margin=0.7in]{geometry}
\usepackage[utf8]{inputenc}
  
\usepackage{amsmath,amssymb,amsfonts,amsthm}

\theoremstyle{definition}
\newtheorem{theorem}{Theorem}

\theoremstyle{definition}
\newtheorem{definition}{Definition}

\newtheorem{corollary}{Corollary}[theorem]
\newtheorem{lemma}{Lemma}

\newenvironment{enumerated}{ 
\begin{enumerate}
\setlength{\itemsep}{0pt}
\setlength{\parskip}{0pt}
\setlength{\parsep}{0pt}     
}{\end{enumerate}} 

\begin{document}

We will first consider the series

$$ \lim_{N \to \infty} \sum_{n=1}^N n(-1)^{n-1} = 1 - 2 + 3 - 4 + 5 - 6 + \cdots $$

Let $s = 1 - 2 + 3 - 4 + \cdots$. Then

$$
\begin{tabular}{l@{ } l@{ } l@{ } l@{ } l}
  $ 4s $ & $ = \ s $ & $ + \ s $ & $ + \ s $ & $ + \ s $ \\
         & $ = (1 - 2 + 3 - 4 + \cdots) $ & $ + \ (1 - 2 + 3 - 4 + \cdots) $ 
         & $ + \ (1 - 2 + 3 - 4 + \cdots) $ & $ + \ (1 - 2 + 3 - 4 + \cdots) $ \\
         & $ = (1 - 2 + 3 - 4 + \cdots) $ & $ + \ 1 + (-2 + 3 -4 + 5 - \cdots) $ 
         & $ + \ 1 + (-2 + 3 -4 + 5 - \cdots) $ & $ + \ (1 - 2) + (3 - 4 + 5 - 6 + \cdots) $ \\
         & $ = (1 - 2 + 3 - 4 + \cdots) $ & $ + \ 1 + (-2 + 3 -4 + 5 - \cdots) $ 
         & $ + \ 1 + (-2 + 3 -4 + 5 - \cdots) $ & $ - \ 1 + (3 - 4 + 5 - 6 + \cdots) $ \\
         & $ = 1 + (1 - 2 + 3 - 4 + \cdots) $ & $ + \ (-2 + 3 -4 + 5 - \cdots) $ 
         & $ + \ (-2 + 3 -4 + 5 - \cdots) $ & $ + \ (3 - 4 + 5 - 6 + \cdots) $ \\
         & $ = 1 + [ \ (1 - 2 - 2 + 3) $ & $ + \ (-2 + 3 + 3 - 4) $ 
         & $ + \ (3 - 4 - 4 + 5) $ & $ + \ (-4 + 5 + 5 - 6) + \cdots \ ] $ \\
         & $ = 1 + [ \ 0 $ & $ + \ 0 $ 
         & $ + \ 0 $ & $ + \ 0 + \cdots \ ] $ \\
         & $ = 1 $
\end{tabular}
$$

So $s = \frac{1}{4}$.

$$
1 + 2 + 3 + 4 + \cdots
$$

\end{document}
